updating tests

coq/examples/test_7.c
@@ -1,0 +1,15 @@
+#include <stdlib.h>
+#include <stdbool.h>
+#include <assert.h>
+
+#include <klee/klee.h>
+
+#define N 10
+
+int main() {
+    int n = 0;
+    while (n < N) {
+        n++;
+    }
+    return 0;
+}
